examples/bug-reports/bug237.fst
@@ -1,0 +1,148 @@
+module Bug236
+
+(* Still can't reproduce this, it only appears in tinyfstar-new.fst *)
+
+open Classical
+
+type var = nat
+
+type typ =
+  | TVar   : a:var -> typ
+  | TConst : typ
+  | TTApp  : t1:typ -> t2:typ -> typ
+
+type knd =
+  | KType : knd
+  | KKArr : karg:knd -> kres:knd -> knd
+  | KTArr : targ:typ -> kres:knd -> knd
+
+type tsub = var -> Tot typ
+opaque type trenaming (s:tsub) = (forall (x:var). is_TVar (s x))
+
+val is_trenaming : s:tsub -> Tot (n:int{(  trenaming s  ==> n=0) /\
+                                        (~(trenaming s) ==> n=1)})
+let is_trenaming s = (if excluded_middle (trenaming s) then 0 else 1)
+
+val tsub_inc_above : nat -> var -> Tot typ
+let tsub_inc_above x y = if y<x then TVar y else TVar (y+1)
+
+val tsub_id :tsub
+let tsub_id = fun x -> TVar x
+
+val tsub_inc : var -> Tot typ
+let tsub_inc = tsub_inc_above 0
+
+let is_tvar (t:typ) : int = if is_TVar t then 0 else 1
+
+(* Can't reproduce it with this
+val ttsubst : s:tsub -> t:typ -> Pure typ (requires True)
+      (ensures (fun t' -> trenaming s /\ is_TVar t ==> is_TVar t'))
+      (decreases %[is_tvar t; is_trenaming s; t])
+val ktsubst : s:tsub -> k:knd -> Tot knd
+      (decreases %[1; is_trenaming s; k])
+
+let rec ttsubst s t =
+  match t with
+  | TVar a -> s a
+  | TConst -> TConst
+  | TTApp t1 t2 -> TTApp (ttsubst s t1) (ttsubst s t2)
+
+and ktsubst s k =
+  match k with
+  | KType -> KType
+  | KKArr k kbody ->
+     let tsub_lam : y :var -> Tot(t:typ{trenaming s ==> is_TVar t}) =
+       fun y -> if y = 0 then TVar y
+                else (ttsubst tsub_inc (s (y-1))) in
+     KKArr (ktsubst s k) (ktsubst tsub_lam kbody)
+  | KTArr t kbody ->
+     KTArr (ttsubst s t) (ktsubst s kbody)
+ *)
+
+(* Can't reproduce it with this either *)
+assume type esub
+assume val esub_id : esub 
+assume val esub_inc : esub
+
+type sub = 
+| Sub : es:esub -> ts:tsub -> sub
+
+assume val esub_tlam: s:sub -> Tot esub
+assume val esub_elam: s:sub -> Tot esub
+
+opaque type renaming (s:sub) = (trenaming (Sub.ts s))
+
+val is_renaming : s:sub -> Tot (n:int{(  renaming s  ==> n=0) /\
+                                       (~(renaming s) ==> n=1)})
+let is_renaming s = (if excluded_middle (renaming s) then 0 else 1)
+
+val tsubst : s:sub -> t:typ -> Pure typ (requires True)
+      (ensures (fun t' -> renaming s /\ is_TVar t ==> is_TVar t'))
+      (decreases %[is_tvar t; is_renaming s;1; t])
+val ksubst : s:sub -> k:knd -> Tot knd
+      (decreases %[1; is_renaming s; 1; k])
+val tsub_elam : s:sub -> a:var -> Tot(t:typ{renaming s ==> is_TVar t}) 
+      (decreases %[1; is_renaming s; 0; TVar 0])
+val tsub_tlam : s:sub -> a:var -> Tot(t:typ{renaming s ==> is_TVar t}) 
+      (decreases %[1; is_renaming s; 0; TVar 0])
+val tsub_elam2 : s:sub -> a:var -> Tot(t:typ{renaming s ==> is_TVar t}) 
+      (decreases %[1; is_renaming s; 0; TVar 0])
+
+let rec tsub_elam s =
+fun a -> tsubst (Sub esub_inc tsub_id) (Sub.ts s a) 
+
+and tsub_tlam s =
+fun a -> if a = 0 then TVar a
+         else tsubst (Sub esub_id tsub_inc) (Sub.ts s a)
+
+and tsub_elam2 s =
+fun a -> tsubst (Sub esub_inc tsub_id) (tsubst (Sub esub_inc tsub_id) (Sub.ts s a))
+
+(*Substitution inside types*)
+and tsubst s t =
+  match t with
+  | TVar a -> (Sub.ts s a)
+  | TConst -> TConst
+  | TTApp t1 t2 -> TTApp (tsubst s t1) (tsubst s t2)
+
+(*Substitution inside kinds*)
+and ksubst s k =
+  match k with
+  | KType -> KType
+  | KKArr k kbody -> 
+     let sub_tlam = Sub (esub_tlam s) (tsub_tlam s) in
+     KKArr (ksubst s k) (ksubst sub_tlam kbody)
+  | KTArr t kbody -> 
+     let sub_elam = Sub (esub_elam s) (tsub_elam s) in
+     (KTArr (tsubst s t) (ksubst sub_elam kbody))
+
+val ktsubst : s:tsub -> k:knd -> Tot knd
+let ktsubst s k = ksubst (Sub esub_id s) k
+
+val tsub_beta_gen : var -> typ -> Tot tsub
+let tsub_beta_gen x t = fun y -> if y < x then (TVar y)
+                                 else if y = x then t
+                                 else (TVar (y-1))
+
+val ktsubst_beta_gen : var -> typ -> knd -> Tot knd
+let ktsubst_beta_gen x t' = ktsubst (tsub_beta_gen x t')
+
+let ktsubst_beta = ktsubst_beta_gen 0
+
+type kinding : g:int -> t:typ -> k:knd -> Type =
+| KConst : g:int ->
+    kinding g TConst (KKArr KType (KKArr (KTArr (TVar 0) KType) KType))
+| KTApp : #g:int -> #t1:typ -> #t2:typ -> #k:knd -> #k':knd ->
+          =hk1:kinding g t1 (KKArr k k') ->
+          =hk2:kinding g t2 k ->
+               (* kinding g (TTApp t1 t2) k' *)
+               kinding g (TTApp t1 t2) (ktsubst_beta t2 k')
+
+val k_foralle : #g:int -> #t1:typ -> #t2:typ ->
+                =hk1:kinding g t1 KType ->
+                Tot (kinding g (TTApp TConst t1)
+                               (KKArr (KTArr t1 KType) KType))
+let k_foralle g t1 t2 hk1 =
+  (* assert(KKArr (KTArr t1 KType) KType =  *)
+  (*        ktsubst_beta t1 (KKArr (KTArr (TVar 0) KType) KType)); *)
+  KTApp (* (KKArr (KTArr (TVar 0) KType) KType) *) (KConst g) hk1
